some fiber bundle stuff, plus reorganizing/reordering topology.lean a bit

gluing.lean
@@ -9,20 +9,25 @@ structure cover (I X : Type) :=
   (part : I → set X)
   (hx : ∀ (x : X), ∃ (i : I), x ∈ part i)
 
+-- coercion so we can write "U i" when (U : cover I X) and (i : I)
+instance cover_to_parts (I X : Type) : has_coe_to_fun (cover I X) :=
+  {F   := λ _, I → set X,
+   coe := λ U, U.part}
+
 -- consistent functions on each part of the cover
 structure gluing_data (I X Y : Type) :=
   (U : cover I X)
-  (f : Π (i : I), (U.part i) → Y)
-  (hglue : ∀ (i j : I) (x : X) (hxi : x ∈ U.part i) (hxj : x ∈ U.part j),
+  (f : Π (i : I), U i → Y)
+  (hglue : ∀ (i j : I) (x : X) (hxi : x ∈ U i) (hxj : x ∈ U j),
     (f i) ⟨x, hxi⟩ = (f j) ⟨x, hxj⟩)
 
 -- what it means for f : X → Y to be compatible with gluing data
-def compatible {I X Y : Type} (gldata : gluing_data I X Y) (f : X → Y) :=
-  ∀ (i : I) (x : X) (hxi : x ∈ gldata.U.part i), f x = gldata.f i ⟨x, hxi⟩
+def compatible {I X Y : Type} (gl : gluing_data I X Y) (f : X → Y) :=
+  ∀ (i : I) (x : X) (hxi : x ∈ gl.U i), f x = gl.f i ⟨x, hxi⟩
 
 lemma compatible_iff_restrict_eq
-  {I X Y : Type} (gldata : gluing_data I X Y) {f : X → Y} :
-  compatible gldata f ↔ ∀ (i : I), subtype.restrict f _ = gldata.f i :=
+  {I X Y : Type} (gl : gluing_data I X Y) {f : X → Y} :
+  compatible gl f ↔ ∀ (i : I), subtype.restrict f _ = gl.f i :=
 begin
   split; intros hf i, specialize hf i,
   ext ⟨x, hx⟩, rw subtype.restrict_apply, exact hf x hx,
@@ -31,23 +36,23 @@ end
 
 -- existence of compatible function
 -- (uses choice, even though the result is unique)
-def mk_function {I X Y : Type} (gldata : gluing_data I X Y) : X → Y :=
-λ x, let ⟨i, hxi⟩ := classical.subtype_of_exists (gldata.U.hx x) in
-  gldata.f i ⟨x, hxi⟩
+def mk_function {I X Y : Type} (gl : gluing_data I X Y) : X → Y :=
+λ x, let ⟨i, hxi⟩ := classical.subtype_of_exists (gl.U.hx x) in
+  gl.f i ⟨x, hxi⟩
 
-lemma mk_compatible {I X Y} (gldata : @gluing_data I X Y) :
-  compatible gldata (mk_function gldata) :=
+lemma mk_compatible {I X Y} (gl : @gluing_data I X Y) :
+  compatible gl (mk_function gl) :=
 begin
   intros i x hxi,
-  let j := classical.subtype_of_exists (gldata.U.hx x),
-  exact gldata.hglue j.val i x j.prop hxi,
+  let j := classical.subtype_of_exists (gl.U.hx x),
+  exact gl.hglue j.val i x j.prop hxi,
 end
 
-lemma compatible_unique {I X Y : Type} (gldata : @gluing_data I X Y) (f g : X → Y) :
-  compatible gldata f → compatible gldata g → f = g :=
+lemma compatible_unique {I X Y : Type} (gl : @gluing_data I X Y) (f g : X → Y) :
+  compatible gl f → compatible gl g → f = g :=
 begin
   intros hf hg,
-  ext, obtain ⟨i, hxi⟩ := gldata.U.hx x,
+  ext, obtain ⟨i, hxi⟩ := gl.U.hx x,
   specialize hf i x hxi,
   specialize hg i x hxi,
   rwa [hf, hg],
@@ -59,7 +64,7 @@ variables
   (I J X Y : Type)
   (CI : cover I X)
   (CJ : cover J X)
-  (gldata : gluing_data I X Y)
+  (gl : gluing_data I X Y)
 
 def refine : cover (I × J) X :=
  ⟨λ ⟨i, j⟩, (CI.part i) ∩ (CJ.part j),
@@ -73,18 +78,18 @@ as the restriction of f from Uᵢ, not Vⱼ.
 -/
 def gl_refine : gluing_data (I × J) X Y :=
   ⟨ -- U, f, hglue
-    refine I J X gldata.U CJ, -- U
+    refine I J X gl.U CJ, -- U
     λ ⟨i, j⟩ ⟨x, hxij⟩,
-    gldata.f i ⟨x, hxij.left⟩,
+    gl.f i ⟨x, hxij.left⟩,
     λ ⟨i₁, j₁⟩ ⟨i₂, j₂⟩ x ⟨hxi₁, hxj₁⟩ ⟨hxi₂, hxj₂⟩,
-    gldata.hglue i₁ i₂ x hxi₁ hxi₂,
+    gl.hglue i₁ i₂ x hxi₁ hxi₂,
   ⟩
 
 variable (f : X → Y)
 
 lemma compat_of_refine_of_compat :
-  compatible gldata f →
-  compatible (gl_refine _ _ _ _ CJ gldata) f :=
+  compatible gl f →
+  compatible (gl_refine _ _ _ _ CJ gl) f :=
 begin
   rintros hf ⟨i, j⟩ x ⟨hxi, hxj⟩,
   exact hf i x hxi,
@@ -107,20 +112,20 @@ instance : has_coe (open_cover I X TX) (cover I X) := ⟨λ U, ⟨U.part, U.hx�
 
 structure cts_gluing_data :=
   (U : open_cover I X TX)
-  (f : Π (i : I), (U.part i) → Y)
-  (hglue : ∀ (i j : I) (x : X) (hxi : x ∈ U.part i) (hxj : x ∈ U.part j),
+  (f : Π (i : I), (U i) → Y)
+  (hglue : ∀ (i j : I) (x : X) (hxi : x ∈ U i) (hxj : x ∈ U j),
     (f i) ⟨x, hxi⟩ = (f j) ⟨x, hxj⟩)
-  (hf : Π (i : I), @cts _ _ (topology.subspace_topology TX (U.part i)) TY (f i))
+  (hf : Π (i : I), @cts _ _ (topology.subspace_topology TX (U i)) TY (f i))
 
 instance : has_coe (cts_gluing_data I X Y TX TY) (gluing_data I X Y) :=
-  ⟨λ gldata, ⟨gldata.U, gldata.f, gldata.hglue⟩⟩
+  ⟨λ gl, ⟨gl.U, gl.f, gl.hglue⟩⟩
 
 variables
-  (U : open_cover I X TX) (gldata : cts_gluing_data I X Y TX TY)
+  (U : open_cover I X TX) (gl : cts_gluing_data I X Y TX TY)
   (f g : X → Y)
 
 lemma cts_iff_cts_on_cover (f : X → Y) : cts TX TY f ↔ 
-  Π (i : I), @cts _ _ (topology.subspace_topology TX (U.part i)) TY
+  Π (i : I), @cts _ _ (topology.subspace_topology TX (U i)) TY
                       (subtype.restrict f _) :=
 begin
   split,
@@ -130,29 +135,78 @@ begin
   rw cts_iff_ptwise_cts, intro x,
   obtain ⟨i, hxi⟩ := U.hx x, specialize hfi i,
   rw cts_iff_ptwise_cts at hfi, specialize hfi ⟨x, hxi⟩,
-  rwa cts_at_pt_of_open TX TY f (U.part i) (U.hopen i) x hxi,
+  rwa cts_at_pt_of_open TX TY f (U i) (U.hopen i) x hxi,
 end
 
 -- function compatible with cts gluing data is cts
 -- (mostly equivalent to cts_iff_cts_on_cover)
 lemma cts_of_cts_compat :
-  compatible (gldata : gluing_data I X Y) f → cts TX TY f :=
+  compatible (gl : gluing_data I X Y) f → cts TX TY f :=
 begin
   intro hf,
-  rw cts_iff_cts_on_cover I X Y TX TY gldata.U,
+  rw cts_iff_cts_on_cover I X Y TX TY gl.U,
   rw compatible_iff_restrict_eq at hf,
-  intro i, specialize hf i, convert gldata.hf i,
+  intro i, specialize hf i, convert gl.hf i,
 end
 
 -- the glued function is continuous! 🎉
-lemma mk_function_cts : cts TX TY (mk_function (gldata : gluing_data I X Y)) :=
-  @cts_of_cts_compat I X Y TX TY gldata
-  (mk_function (gldata : gluing_data I X Y))
-  (mk_compatible ↑gldata)
+lemma mk_function_cts : cts TX TY (mk_function (gl : gluing_data I X Y)) :=
+  @cts_of_cts_compat I X Y TX TY gl
+  (mk_function (gl : gluing_data I X Y))
+  (mk_compatible ↑gl)
 
 section fiber_bundle
 
-parameters 
+def res_l {X Y : Type} {A B : set X} (g : A → Y) : A ∩ B → Y :=
+  λ ⟨a, hab⟩, g ⟨a, hab.1⟩
+
+def res_r {X Y : Type} {A B : set X} (g : B → Y) : A ∩ B → Y :=
+  λ ⟨a, hab⟩, g ⟨a, hab.2⟩
+
+-- collecting the data of a potential bundle
+-- (this definition does not assert any actual properties of π)
+structure prebundle :=
+  (base fiber total_space : Type)
+  (TB : topology base)
+  (TF : topology fiber)
+  (TT : topology total_space)
+  (π : total_space → base)
+  (hπ : function.surjective π ∧ cts TT TB π)
+
+-- what it means for trivialize over a subset
+structure trivialize_subset (E : prebundle) (U : set E.base) :=
+  (φ : U × E.fiber → E.π ⁻¹' U)
+  (hφ_homeo : homeo ↑((E.TB : topology U), E.TF) ↑E.TT φ)
+  (hφ_proj : ∀ u v, E.π (φ ⟨u, v⟩) = u)
+
+-- a fiber bundle together with a choice of trivialization datum
+structure structured_fiber_bundle extends prebundle :=
+  (I : Type)
+  (U : open_cover I base TB)
+  (triv (i : I) : trivialize_subset (to_prebundle) (U i))
+
+-- incomplete, but will likely be needed
+def refine_trivializing
+  (E : prebundle) (U : set E.base) (triv : trivialize_subset E U)
+  (U' : set E.base) (hU' : U' ⊆ U) :
+  trivialize_subset E U' := sorry
+
+
+/- from earlier attempt to define fiber bundle, including transition functions
+  (trans (i j : I) : (U i) ∩ (U j) → fiber → fiber)
+  (htrans (i j : I) :
+    (∀ (u : (U i) ∩ (U j)) (v : fiber),
+      let t := (triv i ⟨⟨u, u.2.1⟩, v⟩) in -- ⟨t.val, h : t ∈ π ⁻¹' U i⟩
+      triv_inv j ⟨t.val, begin simp, rw (htriv i).2.2.2 ⟨u, u.2.1⟩ v, exact u.2.2, end⟩
+        = ⟨⟨u, u.2.2⟩, trans i j u v⟩))
+-/
+
+
+-- This was hard to write -- describing the transition functions especially.
+-- It's annoying to have to coerce between different sets.
+-- I'm not even sure it's complete.
+-- Eventually it will need the transition function to be a rescaling.
+
 
 end fiber_bundle
 
